

1.1.

training data:  $\{(x_1, y_1), (x_2, y_2), \dots, (x_N, y_N)\}$

where:  $x_i \in \mathbb{R}^d, y_i \in \mathbb{R}^k$  for  $i = 1, 2, \dots, N$

consider:  $\min_{w \in \mathbb{R}^{k \times d}, b \in \mathbb{R}^k} \sum_{i=1}^N \|y_i - wx_i - b\|_2^2$  (least-square problem)

Q1: set  $\tilde{x}_i = \begin{bmatrix} x_i \\ 1 \end{bmatrix} \in \mathbb{R}^{d+1}$

$\tilde{w} = [w | b] \in \mathbb{R}^{k \times (d+1)}$

then origin question  $\Leftrightarrow \min_{\tilde{w}} \sum_{i=1}^N \|y_i - \tilde{w} \tilde{x}_i\|_2^2$

set  $X = \begin{bmatrix} \tilde{x}_1^T \\ \tilde{x}_2^T \\ \vdots \\ \tilde{x}_N^T \end{bmatrix} = \begin{bmatrix} x_1^T & 1 \\ x_2^T & 1 \\ \vdots & \vdots \\ x_N^T & 1 \end{bmatrix} \in \mathbb{R}^{N \times (d+1)}; Y = \begin{bmatrix} y_1^T \\ y_2^T \\ \vdots \\ y_N^T \end{bmatrix} \in \mathbb{R}^{N \times k}$

then  $L(\tilde{w}) = \|Y - X\tilde{w}\|_F^2 = \text{tr}((Y - X\tilde{w})(Y - X\tilde{w})^T)$   
 $= \text{tr}(Y^T Y) - 2\text{tr}(Y^T X\tilde{w}) + \text{tr}(\tilde{w}^T X^T X \tilde{w})$

$\therefore \frac{\partial L}{\partial \tilde{w}} = -2(Y^T X)^T + 2(X^T X \tilde{w})^T = -2X^T Y + 2X^T X \tilde{w}^T$

let  $\frac{\partial L}{\partial \tilde{w}} = 0 \Rightarrow -2X^T Y + 2X^T X \tilde{w}^T = 0$   
 $\Rightarrow X^T X \tilde{w}^T = X^T Y$

assume  $X^T X$  is invertible then

$\tilde{w}^T = (X^T X)^{-1} X^T Y$

$\therefore \tilde{w} = [w | b]$

$\therefore w^* = \tilde{w}[:, 1:d], b^* = \tilde{w}[:, d]$

where  $\tilde{w}^T = (X^T X)^{-1} X^T Y \in \mathbb{R}^{(d+1) \times k}$

$\therefore$  final closed form  
 $\begin{bmatrix} w^* \\ b^* \end{bmatrix} = (X^T X)^{-1} X^T Y \in \mathbb{R}^{(d+1) \times k}$  where  $X = \begin{bmatrix} \tilde{x}_1^T \\ \tilde{x}_2^T \\ \vdots \\ \tilde{x}_N^T \end{bmatrix} = \begin{bmatrix} x_1^T & 1 \\ x_2^T & 1 \\ \vdots & \vdots \\ x_N^T & 1 \end{bmatrix} \in \mathbb{R}^{N \times (d+1)}; Y = \begin{bmatrix} y_1^T \\ y_2^T \\ \vdots \\ y_N^T \end{bmatrix} \in \mathbb{R}^{N \times k}$

Q2:

for a single sample  $(x_i, y_i)$ , the loss is

$\mathcal{L}_i(w, b) = \|y_i - wx_i - b\|_2^2 = (y_i - wx_i - b)^T (y_i - wx_i - b)$

we have

$\frac{\partial \mathcal{L}_i}{\partial w} = -2(y_i - wx_i - b)x_i^T; \frac{\partial \mathcal{L}_i}{\partial b} = -2(y_i - wx_i - b)$

$\therefore \frac{\partial L}{\partial w} = -2 \sum_{i=1}^N (y_i - wx_i - b)x_i^T$  and  $\frac{\partial L}{\partial b} = -2 \sum_{i=1}^N (y_i - wx_i - b)$

$\Rightarrow$  At iteration  $t$ , we have

$w^{(t+1)} = w^{(t)} + 2\eta \sum_{i=1}^N (y_i - w^{(t)}x_i - b^{(t)})x_i^T$

$b^{(t+1)} = b^{(t)} + 2\eta \sum_{i=1}^N (y_i - w^{(t)}x_i - b^{(t)})$

where  $\eta > 0$  is the learning rate.

in matrix form.

Gradient:  $\frac{\partial L}{\partial w} = -2X^T(Y - X\tilde{w}^{(t)})$

Update rule:  $\tilde{w}^{(t+1)T} = \tilde{w}^{(t)T} + 2\eta X^T(Y - X\tilde{w}^{(t)T})$

Stopping Criteria

1. Stop when the gradient norm is small enough:

$\|\frac{\partial L}{\partial \tilde{w}}\|_F < \epsilon_g$

2. Stop when the change in loss between consecutive iteration is small enough

$|L(w^{(t+1)}, b^{(t+1)}) - L(w^{(t)}, b^{(t)})| < \epsilon_L$  or  $\frac{|L^{(t)} - L^{(t+1)}|}{|L^{(t)} + \epsilon_L|} < \epsilon_L$

Q3.

consider loss for single sample

$$\ell_i(W) = -\sum_{k=1}^K y_{i,k} \log(\hat{y}_{i,k})$$

then  $\frac{\partial \ell_i}{\partial W} = \frac{\partial \ell_i}{\partial z_i} \cdot \frac{\partial z_i}{\partial W}$

where  $\frac{\partial \ell_i}{\partial z_{i,k}} = -\sum_{j=1}^K y_{i,j} \frac{\partial \log(\hat{y}_{i,j})}{\partial z_{i,k}}$

for  $\frac{\partial \hat{y}_{i,j}}{\partial z_{i,k}}$  when  $j=k$ ,  $\frac{\partial \hat{y}_{i,j}}{\partial z_{i,k}} = \hat{y}_{i,k}(1 - \hat{y}_{i,k})$

when  $j \neq k$ ,  $\frac{\partial \hat{y}_{i,j}}{\partial z_{i,k}} = -\hat{y}_{i,j} \hat{y}_{i,k}$  for softmax

combined, we have

$$\frac{\partial \ell_i}{\partial z_{i,k}} = \hat{y}_{i,j} (\delta_{jk} - \hat{y}_{i,k}) \text{ where } \delta_{jk} \text{ is the Kronecker delta.}$$

$$\therefore \frac{\partial \ell_i}{\partial z_{i,k}} = -\sum_{j=1}^K y_{i,j} \frac{1}{\hat{y}_{i,j}} \frac{\partial \hat{y}_{i,j}}{\partial z_{i,k}}$$

$$= -\sum_{j=1}^K y_{i,j} \frac{1}{\hat{y}_{i,j}} (\delta_{jk} - \hat{y}_{i,k}) \cdot \hat{y}_{i,j}$$

$$= -\sum_{j=1}^K y_{i,j} (\delta_{jk} - \hat{y}_{i,k})$$

$$= -\sum_{j=1}^K y_{i,j} \delta_{jk} + \sum_{j=1}^K y_{i,j} \hat{y}_{i,k}$$

$$= -y_{i,k} + \hat{y}_{i,k} \sum_{j=1}^K y_{i,j}$$

$\because y_i$  is one-hot encoded ( $\sum_{j=1}^K y_{i,j} = 1$ )

$$\therefore \frac{\partial \ell_i}{\partial z_{i,k}} = \hat{y}_{i,k} - y_{i,k}$$

in vector form

$$\frac{\partial \ell_i}{\partial z_i} = \hat{y}_i - y_i$$

$$\because z_i = W^T x_i$$

$$\therefore z_{i,k} = \sum_{m=1}^d W_{m,k} x_{i,m}$$

$$\therefore \frac{\partial z_{i,k}}{\partial W_{m,n}} = x_{i,m} \delta_{kn}$$

in matrix form

$$\frac{\partial z_i}{\partial W} = x_i \otimes I_k \text{ where } \otimes \text{ is the outer product.}$$

$$\therefore \frac{\partial \ell_i}{\partial W} = x_i (\hat{y}_i - y_i)^T$$

$$\therefore \frac{\partial J}{\partial W} = \frac{1}{N} \sum_{i=1}^N \frac{\partial \ell_i}{\partial W}$$

$$= \frac{1}{N} \sum_{i=1}^N x_i (\hat{y}_i - y_i)^T$$

set  $X = \begin{bmatrix} x_1^T \\ x_2^T \\ \vdots \\ x_N^T \end{bmatrix} = R^{N \times d}$ ;  $Y = \begin{bmatrix} y_1^T \\ y_2^T \\ \vdots \\ y_N^T \end{bmatrix} \in R^{N \times k}$ ,  $\hat{Y} = \begin{bmatrix} \hat{y}_1^T \\ \hat{y}_2^T \\ \vdots \\ \hat{y}_N^T \end{bmatrix}$

then  $\sum_{i=1}^N x_i (\hat{y}_i - y_i)^T = X^T (\hat{Y} - Y)$

$$\therefore \nabla_W J = \frac{1}{N} X^T (\hat{Y} - Y)$$

1.2.

Q1.

Slack Variables

$\epsilon_i \geq 0$ : measures the violation when  $y_i - f(x_i) > \epsilon$

$\epsilon_i^* \geq 0$ : measures the violation when  $f(x_i) - y_i > \epsilon$

$\therefore$  origin problem becomes:  $\min_{w, \epsilon, \epsilon^*} \frac{1}{2} \|w\|^2 + C \sum_{i=1}^n (\epsilon_i + \epsilon_i^*)$

Subject to

$$y_i - w^T x_i \leq \epsilon + \xi_i^*$$

$$w^T x_i - y_i \leq \epsilon + \xi_i$$

Q2.

introduce

$\alpha_i \geq 0$  for constraints  $w^T x_i - y_i \leq \epsilon + \xi_i$

$\alpha_i^* \geq 0$  for constraints  $y_i - w^T x_i \leq \epsilon + \xi_i^*$

$\lambda_i \geq 0$  for constraints  $\xi_i \geq 0$

$\lambda_i^* \geq 0$  for constraints  $\xi_i^* \geq 0$

$$\therefore L(w, \epsilon, \xi, \alpha, \alpha^*, \lambda, \lambda^*) = \frac{1}{2} \|w\|^2 + C \sum_{i=1}^n (\xi_i + \xi_i^*)$$

$$+ \sum_{i=1}^n \alpha_i (w^T x_i - y_i - \epsilon - \xi_i)$$

$$+ \sum_{i=1}^n \alpha_i^* (w^T x_i - y_i - \epsilon - \xi_i^*)$$

$$- \sum_{i=1}^n \lambda_i \xi_i - \sum_{i=1}^n \lambda_i^* \xi_i^*$$

Q3.

We have

$$L(w, \epsilon, \xi, \alpha, \alpha^*, \lambda, \lambda^*) = \frac{1}{2} \|w\|^2 + C \sum_{i=1}^n (\xi_i + \xi_i^*)$$

$$+ \sum_{i=1}^n \alpha_i (w^T x_i - y_i - \epsilon - \xi_i)$$

$$+ \sum_{i=1}^n \alpha_i^* (w^T x_i - y_i - \epsilon - \xi_i^*)$$

$$- \sum_{i=1}^n \lambda_i \xi_i - \sum_{i=1}^n \lambda_i^* \xi_i^*$$

$\therefore$  KKT

$$\therefore \frac{\partial L}{\partial w} = w + \sum_{i=1}^n \alpha_i x_i - \sum_{i=1}^n \alpha_i^* x_i = 0$$

$$\Rightarrow w = \sum_{i=1}^n (\alpha_i^* - \alpha_i) x_i$$

$$\frac{\partial L}{\partial \xi_i} = C - \alpha_i - \lambda_i = 0$$

$$\Rightarrow C = \alpha_i + \lambda_i$$

$$\frac{\partial L}{\partial \xi_i^*} = C - \alpha_i^* - \lambda_i^* = 0$$

$$\Rightarrow C = \alpha_i^* + \lambda_i^*$$

$$\therefore \alpha_i (w^T x_i - y_i - \epsilon - \xi_i) = 0$$

$$\alpha_i^* (y_i - w^T x_i - \epsilon - \xi_i^*) = 0$$

$$\lambda_i \xi_i = 0$$

$$\lambda_i^* \xi_i^* = 0$$

$$\therefore \frac{1}{2} \|w\|^2 = \frac{1}{2} \left\| \sum_{i=1}^n (\alpha_i^* - \alpha_i) x_i \right\|^2 = \frac{1}{2} \sum_{i,j=1}^n (\alpha_i^* - \alpha_i) (\alpha_j^* - \alpha_j) x_i^T x_j$$

$$\therefore C = \alpha_i + \lambda_i \quad C = \alpha_i^* + \lambda_i^*$$

$$\therefore \left( \sum_{i=1}^n (\xi_i + \xi_i^*) - \sum_{i=1}^n \lambda_i \xi_i - \sum_{i=1}^n \lambda_i^* \xi_i^* \right) = \sum_{i=1}^n \alpha_i \xi_i + \sum_{i=1}^n \alpha_i^* \xi_i^*$$

$$\therefore L = - \frac{1}{2} \sum_{i,j=1}^n (\alpha_i - \alpha_i^*) (\alpha_j - \alpha_j^*) x_i^T x_j + \sum_{i=1}^n (\alpha_i^* - \alpha_i) y_i - \epsilon \sum_{i=1}^n (\alpha_i + \alpha_i^*)$$

$\therefore$  we have Dual Form of SVR

Maximize

$$L_D(\alpha, \alpha^*) = - \frac{1}{2} \sum_{i,j=1}^n (\alpha_i - \alpha_i^*) (\alpha_j - \alpha_j^*) x_i^T x_j + \sum_{i=1}^n (\alpha_i^* - \alpha_i) y_i - \epsilon \sum_{i=1}^n (\alpha_i + \alpha_i^*)$$

Subject to:

$$0 \leq \alpha_i \leq C, i=1, \dots, n$$

$$0 \leq \alpha_i^* \leq C, i=1, \dots, n$$

Using  $w = \sum_{i=1}^n (\alpha_i^* - \alpha_i) x_i$  we have  $f(x) = \sum_{i=1}^n (\alpha_i^* - \alpha_i) x_i^T x$

Q4. yes:

Dual Problem rewritten:

Minimize

$$\frac{1}{2} \sum_{i,j=1}^n (\alpha_i - \alpha_i^*) (\alpha_j - \alpha_j^*) x_i^T x_j - \sum_{i=1}^n (\alpha_i^* - \alpha_i) y_i + \epsilon \sum_{i=1}^n (\alpha_i + \alpha_i^*)$$

Subject to:

$$0 \leq \alpha_i \leq C, i=1, \dots, n$$

$$0 \leq \alpha_i^* \leq C, i=1, \dots, n$$

We define

$$u = [\alpha_1 \dots \alpha_n, \alpha_1^* \dots, \alpha_n^*]^T \in \mathbb{R}^{2n}$$

$$Q = \begin{bmatrix} K & -K \\ -K & K \end{bmatrix} \text{ where } K_{ij} = x_i^T x_j$$

$$p = [-y_1 + \epsilon, \dots, -y_n + \epsilon, y_1 + \epsilon, \dots, y_n + \epsilon]^T$$

then we have

$$\min \frac{1}{2} u^T Q u + p^T u$$

subject to

$$0 \leq u \leq C \mathbf{1}$$

Q5.

define margin Support Vectors:

Points where  $0 < \alpha_i < C$  or  $0 < \alpha_i^* < C$

$$\text{For } \alpha_i > 0, w^T x_i - y_i = \epsilon$$

$$\text{For } \alpha_i^* > 0, y_i - w^T x_i = \epsilon$$

$$\text{and } |f(x_i) - y_i| = \epsilon$$

$\because K \neq T$

$$\therefore \alpha_i > 0, w^T x_i - y_i = \epsilon + \epsilon_i$$

$$\alpha_i^* > 0, y_i - w^T x_i = \epsilon + \epsilon_i^*$$

$$\text{for } 0 < \alpha_i < C, \epsilon_i = 0$$

$$\text{for } \alpha_i = C, \epsilon_i > 0$$

$$\begin{array}{c} \bullet \alpha_i^* = C \\ \bullet 0 < \alpha_i < C \\ \text{regression line} \\ f(x) \quad \text{---} \quad f(x) + \epsilon \\ \text{---} \quad f(x) - \epsilon \\ \bullet 0 < \alpha_i^* < C \\ \bullet \alpha_i = C \end{array}$$